src/Exp.v
@@ -36,8 +36,6 @@ Inductive Exp Γ : Ty → Type :=
 
   (* | Builtin {τ ty} : Exp Γ ty → Exp (ty :: Γ) τ → Exp Γ τ *)
 
-  | Let {τ ty}    : Exp Γ ty → Exp (ty :: Γ) τ → Exp Γ τ
-
   (* These are the terms of the base lambda calculus *)
   | VAR {τ}       : Var Γ τ → Exp Γ τ
   | LAM {dom cod} : Exp (dom :: Γ) cod → Exp Γ (dom ⟶ cod)
@@ -58,7 +56,6 @@ Fixpoint Exp_size {Γ τ} (e : Exp Γ τ) : nat :=
   | Fst _ p      => 1 + Exp_size p
   | Snd _ p      => 1 + Exp_size p
   | Seq _ x y    => 1 + Exp_size x + Exp_size y
-  | Let _ x body => 1 + Exp_size x + Exp_size body
   | VAR _ v      => 1
   | LAM _ e      => 1 + Exp_size e
   | APP _ e1 e2  => 1 + Exp_size e1 + Exp_size e2
@@ -92,7 +89,6 @@ Arguments Pair {Γ τ1 τ2} _ _.
 Arguments Fst {Γ τ1 τ2} _.
 Arguments Snd {Γ τ1 τ2} _.
 Arguments Seq {Γ τ τ'} _ _.
-Arguments Let {Γ τ ty} _ _.
 Arguments VAR {Γ τ} _.
 Arguments LAM {Γ dom cod} _.
 Arguments APP {Γ dom cod} _ _.
